Add a few more example proofs

src/example.lean
@@ -9,6 +9,7 @@ def X : finset ℕ := {1}
 def Y : finset ℕ := {2}
 def Z : finset ℕ := {3}
 
+@[simp]
 def var' (n : ℕ) : exp {n} :=
   var ⟨n, finset.mem_insert_self n ∅⟩
 
@@ -27,14 +28,48 @@ def G : subst Y Z := sub 2 3
 example : subst.apply F (var' 1) = var' 2 := rfl
 example : subst.apply G (var' 2) = var' 3 := rfl
 example : subst.apply G (subst.apply F (var' 1)) = var' 3 := rfl
+example : subst.apply G (subst.apply F (var' 1)) = subst.apply (subst.apply G ∘ F) (var' 1) := rfl
 
 def v1 : exp X := lam' 2 (insert_var 2 (var' 1))
 example : subst.apply F v1 = lam' 3 (insert_var 3 (var' 2)) := rfl
 example : subst.apply G (subst.apply F v1) = lam' 4 (insert_var 4 (var' 3)) := rfl
+example : subst.apply G (subst.apply F v1) = subst.apply (subst.apply G ∘ F) v1 := by refl
+example : subst.apply (subst.update (fresh X).1 (fresh Y).1 F) (insert_var (fresh X).1 v1) = lam' 4 (var ⟨2, _⟩) := rfl
+example : insert_var (fresh Y).1 (subst.apply F v1) = lam' 3 (var ⟨2, _⟩) := rfl
+example : subst.apply (subst.update (fresh X).1 (fresh Y).1 F) (insert_var (fresh X).1 v1) ≡α⟨vrel.id (insert (fresh Y).1 Y)⟩ insert_var (fresh Y).1 (subst.apply F v1) :=
+  begin
+    simp [v1],
+    rw [insert_var.lam_comp (insert_var 2 (var ⟨1, _⟩)), subst.apply, subst.apply],
+    rw insert_var.lam_self (subst.apply (subst.update 2 ((fresh Y).fst) F) (insert_var 2 (var ⟨1, _⟩))),
+    apply aeq.lam,
+    rw [insert_var.var, insert_var.var, map, subst.apply, subst.apply, vname.insert, vname.insert, vname.map_of_subset],
+    simp [subst.update],
+    have one_ne_two : 1 ≠ 2 := dec_trivial,
+    rw dif_neg one_ne_two,
+    have p : (fresh X).1 = 2 := rfl, rw p, clear p,
+    rw dif_neg one_ne_two,
+    have p : (fresh Y).1 = 3 := rfl, rw p, clear p,
+    have p : (fresh (insert 3 Y)).1 = 4 := rfl, rw p, clear p,
+    simp [vname.erase],
+    have p : F ⟨1, _⟩ = var ⟨2, _⟩ := rfl, rw p, clear p,
+    simp [insert_var.var],
+    apply aeq.var,
+    simp [vrel.update],
+    right,
+    rw [vname.insert, vname.insert, vname.insert],
+    have two_ne_four : 2 ≠ 4 := dec_trivial,
+    existsi two_ne_four,
+    have two_ne_three : 2 ≠ 3 := dec_trivial,
+    existsi two_ne_three,
+    simp [vname.erase, vrel.id]
+  end
 
-def v2 : exp ∅ := lam' 1 (var' 1)
-example : insert_var 1 v2 = lam' 1 (insert_var 1 (var' 1)) := rfl
-example : subst.apply F (insert_var 1 v2) = lam' 3 (var (vname.insert_self 3 Y)) := rfl
-example : subst.apply G (subst.apply F (insert_var 1 v2)) = lam' 4 (var (vname.insert_self 4 Z)) := rfl
+def v2 : exp X := insert_var 1 (lam' 1 (var' 1))
+example : subst.apply F v2 = lam' 3 (var (vname.insert_self 3 Y)) := rfl
+example : subst.apply G (subst.apply F v2) = lam' 4 (var (vname.insert_self 4 Z)) := rfl
+example : subst.apply (subst.apply G ∘ F) v2 = lam' 4 (var (vname.insert_self 4 Z)) := rfl
+example : subst.apply G (subst.apply F v2) = subst.apply (subst.apply G ∘ F) v2 := by refl
+example : subst.apply (subst.update (fresh X).1 (fresh Y).1 F) (insert_var (fresh X).1 v2) = lam' 4 (var (vname.insert_self 4 (insert (fresh Y).1 Y))) := rfl
+example : insert_var (fresh Y).1 (subst.apply F v2) = lam' 3 (var (vname.insert_self 3 (insert (fresh Y).1 Y))) := rfl
 
 end /- namespace -/ acie -------------------------------------------------------
